TransformExpr lifted stmts

deps/poulet4/lib/P4cub/Transformations/Lifted.v
@@ -28,6 +28,90 @@ Section Lifted.
       lifted_expr e ->
       lifted_expr <{ Access e[z] @ i }>.
 
+  Inductive lifted_args : E.arrowE tags_t -> Prop :=
+  | lifted_args_arrow tes teo :
+      F.predfs_data (P4cub.pred_paramarg_same (lifted_expr ∘ snd)) tes ->
+      predop (lifted_expr ∘ snd) teo ->
+      lifted_args (P4cub.Arrow tes teo).
+  
+  Inductive lifted_stmt : ST.s tags_t -> Prop :=
+  | lifted_skip i :
+      lifted_stmt -{ skip @ i }-
+  | lifted_vardecl x τ i :
+      lifted_stmt -{ var x:τ @ i }-
+  | lifted_assign τ e1 e2 i :
+      lifted_expr e1 ->
+      lifted_expr e2 ->
+      lifted_stmt -{ asgn e1 := e2:τ @ i }-
+  | lifted_bit x w n τ τx i ix iw :
+      lifted_stmt -{ asgn Var x:τx @ ix := w W n @ iw : τ @ i }-
+  | lifted_int x w z τ τx i ix iw :
+      lifted_stmt -{ asgn Var x:τx @ ix := w S z @ iw : τ @ i }-
+  | lifted_uop op x e τ τx τe i ix ie :
+      lifted_expr e ->
+      lifted_stmt -{ asgn Var x:τx @ ix := UOP op e:τe @ ie :τ @ i}-
+  | lifted_bop op x e1 e2 τ τx τ1 τ2 i ix ie1e2 :
+      lifted_expr e1 ->
+      lifted_expr e2 ->
+      lifted_stmt
+      -{ asgn Var x:τx @ ix := BOP e1:τ1 op e2:τ2 @ ie1e2 : τ @ i }-
+  | lifted_slice x e hi lo τ τx τe i ix ie :
+      lifted_expr e ->
+      lifted_stmt
+      -{ asgn Var x:τx @ ix := Slice e:τe [hi:lo] @ ie : τ @ i }-
+  | lifted_cast x e τ τx τe i ix ie :
+      lifted_expr e ->
+      lifted_stmt -{ asgn Var x:τx @ ix := Cast e:τe @ ie : τ @ i }-
+  | lifted_tuple x es τ τx i ix ies :
+      Forall lifted_expr es ->
+      lifted_stmt -{ asgn Var x:τx @ ix := tup es @ ies : τ @ i }-
+  | lifted_struct x es τ τx i ix ies :
+      F.predfs_data (lifted_expr ∘ snd) es ->
+      lifted_stmt -{ asgn Var x:τx @ ix := struct { es } @ ies : τ @ i }-
+  | lifted_header x e es τ τx i ix ies :
+      lifted_expr e ->
+      F.predfs_data (lifted_expr ∘ snd) es ->
+      lifted_stmt
+      -{ asgn Var x:τx @ ix := hdr { es } valid:=e @ ies : τ @ i }-
+  | lifted_stack x es n ni τ τx τs i ix ies :
+      Forall lifted_expr es ->
+      lifted_stmt
+      -{ asgn Var x:τx @ ix
+         := Stack es:τs[n] nextIndex:=ni @ ies : τ @ i }-
+  | lifted_cond e s1 s2 i :
+      lifted_expr e ->
+      lifted_stmt s1 ->
+      lifted_stmt s2 ->
+      lifted_stmt -{ if e then s1 else s2 @ i }-
+  | lifted_seq s1 s2 i :
+      lifted_stmt s1 ->
+      lifted_stmt s2 ->
+      lifted_stmt -{ s1; s2 @ i }-
+  | lifted_block s :
+      lifted_stmt s ->
+      lifted_stmt -{ b{ s }b }-
+  | lifted_extern_method_call e f targs args i :
+      lifted_args args ->
+      lifted_stmt (ST.SExternMethodCall e f targs args i)
+  | lifted_fun_call f targs args i :
+      lifted_args args ->
+      lifted_stmt (ST.SFunCall f targs args i)
+  | lifted_act_call a args i :
+      F.predfs_data (P4cub.pred_paramarg_same (lifted_expr ∘ snd)) args ->
+      lifted_stmt -{ calling a with args @ i }-
+  | lifted_return_void i :
+      lifted_stmt -{ returns @ i }-
+  | lifted_return_fruit τ e i :
+      lifted_expr e ->
+      lifted_stmt -{ return e:τ @ i }-
+  | lifted_exit i :
+      lifted_stmt -{ exit @ i }-
+  | lifted_invoke t i :
+      lifted_stmt -{ invoke t @ i }-
+  | lifted_apply x ext_args args i :
+      F.predfs_data (P4cub.pred_paramarg_same (lifted_expr ∘ snd)) args ->
+      lifted_stmt -{ apply x with ext_args & args @ i }-.
+  
   Local Hint Constructors lifted_expr : core.
 
   Ltac transformExpr_destr :=
@@ -39,9 +123,23 @@ Section Lifted.
   Ltac transformExpr_destr_hyp :=
     match goal with
     | H: context [TransformExpr _ ?e ?env] |- _
-      => destruct (TransformExpr _ e env) as [[? ?] ?] eqn:?; simpl in *
+      => destruct (TransformExpr _ e env)
+        as [[? ?] ?] eqn:?; simpl in *
     end.
 
+  Ltac transformExpr_destr_hyp_rewrite :=
+    match goal with
+    | H: TransformExpr _ ?e ?env = (_,_,_),
+         Hy : context [TransformExpr _ ?e ?env]
+      |- _ => rewrite H in Hy; simpl in *
+    end.
+
+  (*Ltac quantify_varNameGen :=
+    match goal with
+    | env: VarNameGen.t, H: (forall _: VarNameGen.t, _)
+      |- _ => specialize H with env
+    end.*)
+  
   Ltac fold_destr :=
     match goal with
     | |- context [fold_left ?f ?l ?acc]
@@ -50,9 +148,7 @@ Section Lifted.
       => destruct (fold_right f acc l) as [[? ?] ?] eqn:Hfoldl; simpl in *
     end.
   
-  (*Arguments VarNameGen.new_var env : simpl never.*)
-  
-  Lemma TransformExpr_lifted : forall e env,
+  Lemma TransformExpr_lifted_expr : forall e env,
       lifted_expr (snd (fst (TransformExpr _ e env))).
   Proof.
     intro e; induction e using custom_e_ind;
@@ -71,4 +167,44 @@ Section Lifted.
         try (constructor; specialize IHe with env;
              transformExpr_destr_hyp; inv Heqp; auto; assumption).
   Qed.
+
+  Local Hint Constructors lifted_stmt : core.
+
+  Ltac seq_lift :=
+    match goal with
+    | |- lifted_stmt -{ _; _ @ _ }-
+      => apply lifted_seq
+    end.
+
+  Local Hint Resolve TransformExpr_lifted_expr : core.
+  
+  Lemma TransformExpr_lifted_stmt : forall e env,
+      lifted_stmt (fst (fst (TransformExpr _ e env))).
+  Proof.
+    intro e; induction e using custom_e_ind;
+      intro env; unravel in *;
+        repeat transformExpr_destr;
+        repeat seq_lift; auto;
+          try (specialize IHe with env;
+               transformExpr_destr_hyp_rewrite;
+               assumption);
+          try (specialize IHe with env;
+               transformExpr_destr_hyp_rewrite;
+               apply f_equal with (f:= (snd ∘ fst)) in Heqp;
+               unravel in *; rewrite <- Heqp; auto; assumption).
+    - specialize IHe1 with env;
+        transformExpr_destr_hyp_rewrite; assumption.
+    - specialize IHe2 with t;
+        transformExpr_destr_hyp_rewrite; assumption.
+    - specialize IHe1 with env;
+        specialize IHe2 with t;
+        transformExpr_destr_hyp_rewrite;
+        apply f_equal with (f:= (snd ∘ fst)) in Heqp;
+        apply f_equal with (f:= (snd ∘ fst)) in Heqp0.
+      unravel in *; rewrite <- Heqp, <- Heqp0; auto.
+    - admit.
+    - admit.
+    - admit.
+    - admit. 
+  Admitted.
 End Lifted.
